fix start_function

src/Core/StructNormalizer.v
@@ -14,41 +14,49 @@ Fixpoint find_struct_fields (id : ident) (c : list composite_definition) :=
 Fixpoint ls_to_seq (ls : list statement) :=
   match ls with
   | [] => Sskip
-  | [h] => h
+  | [h] => hx
   | h1 :: h2 :: tl => Ssequence h1 (Ssequence h2 (ls_to_seq tl))
   end.
 
-Fixpoint copy_by_fields (p : positive) (id1 id2 : ident) (ty : type) (ls : members) :=
+Fixpoint copy_by_fields (p : positive) (e : expr) (id2 : ident) (ty : type) (ls : members) :=
   match ls with
   | [] => []
   | h :: tl => let f := fst h in
              let t := snd h in
-             let s := Ssequence
-                        (Sset p (Efield (Evar id2 ty) f t))
-                        (Sassign  (Efield (Ederef (Etempvar id1 (tptr ty)) ty) f t) (Etempvar p t))
-             in
-             s :: copy_by_fields (p + 1)%positive id1 id2 ty tl
+             let s :=
+                 Ssequence
+                   (Sset p (Efield (Evar id2 ty) f t))
+              match e with 
+                | (Evar id1 ty1) => (Sassign (Efield (Evar id1 (tptr ty)) f t) (Etempvar p t))
+                | (Etempvar id1 ty1) => (Sassign (Efield (Etempvar id1 (tptr ty)) f t) (Etempvar p t))
+                | (Ederef (Evar id1 ty1) _)  (* cannot happen? *)
+                | (Ederef (Etempvar id1 ty1) _) => (Sassign  (Efield (Ederef (Etempvar id1 (tptr ty)) ty) f t) (Etempvar p t))
+                | _ => Sskip
+              end in
+             s :: copy_by_fields (p + 1)%positive e id2 ty tl
   end.
 
-Fixpoint struct_normalize (s : statement) (c : list composite_definition) :=
+Fixpoint struct_normalize (s : statement) (c : list composite_definition) (p : positive) :=
   match s with
-  | Ssequence s1 s2 => Ssequence (struct_normalize s1 c) (struct_normalize s2 c)
-  | Sloop s1 s2 => Sloop (struct_normalize s1 c) (struct_normalize s2 c)
-  | Sifthenelse e s1 s2 => Sifthenelse e (struct_normalize s1 c) (struct_normalize s2 c)
+  | Ssequence s1 s2 => Ssequence (struct_normalize s1 c p) (struct_normalize s2 c p)
+  | Sloop s1 s2 => Sloop (struct_normalize s1 c p) (struct_normalize s2 c p)
+  | Sifthenelse e s1 s2 => Sifthenelse e (struct_normalize s1 c p) (struct_normalize s2 c p)
   | Sswitch e ls => Sswitch e ((fix switch_normalize ls :=
                                  match ls with
                                  | LSnil => LSnil
-                                 | LScons z s ls' => LScons z (struct_normalize s c) (switch_normalize ls')
+                                 | LScons z s ls' => LScons z (struct_normalize s c p) (switch_normalize ls')
                                  end) ls)
-  | Slabel l s => Slabel l (struct_normalize s c)
-  | Sassign (Evar id1 ty1) (Evar id2 ty2)
-  | Sassign (Etempvar id1 ty1) (Evar id2 ty2)
-  | Sassign (Ederef (Evar id1 ty1) _) (Evar id2 ty2)
-  | Sassign (Ederef (Etempvar id1 ty1) _) (Evar id2 ty2) =>
+  | Slabel l s => Slabel l (struct_normalize s c p)
+  | Sassign e (Evar id2 ty2) =>
     match ty2 with
-      | Tstruct _struct _ => let ls := find_struct_fields _struct c in 
-                            ls_to_seq (copy_by_fields 900%positive id1 id2 (Tstruct _struct noattr) ls)
-      | _ => s
+    | Tstruct _struct _ => let ls := find_struct_fields _struct c in 
+                           ls_to_seq (copy_by_fields p e id2 (Tstruct _struct noattr) ls)
+    | _ => s
     end
   | s => s 
   end.
+
+
+Definition normalize_function f c :=
+  mkfunction (fn_return f) (fn_callconv f) (fn_params f) (fn_vars f) (fn_temps f)
+             (struct_normalize (fn_body f) c).
